\documentclass[11pt, a4paper, oneside]{article}

\begin{document}
\title{Fourth Problem Set}
\author{Aaron Rosen}
\date{Friday, February 22}
\maketitle

\section*{Problem 1}
$B \models C$ just in case $\models (B \to C)$ \\
just in case $\bar{v}(B \to C) = T$ \\
just in case \\
$\bar{v}(B) = T$ and $\bar{v}(C) = T$ \\
or \\
$\bar{v}(B) = F$ and $\bar{v}(C) = T$ \\
or \\
$\bar{v}(B) = F$ and $\bar{v}(C) = F$ \\
In the second two cases, $\bar{v}(B) = F$ 
   which means $\bar{v}(\neg{B}) = T$\\ 
Hence $\models \neg{B}$\\
In the first two cases $\bar{v}(C) = T$ which means $\models C$\\
So in all three cases $\models \neg{b}$ or $\models C$.


\section*{Problem 2}
\subsection*{(a)}
$(x \land y \land \neg{z}) \lor (x \land \neg{y} \land z) 
   \lor (\neg{x} \land y \land z) \lor (\neg{x} \land y \land \neg{z})
   \lor (\neg{x} \land \neg{y} \land \neg{z})$

\subsection*{(b)}
$\neg{(x \land y \land z)} \land \neg{(x \land \neg{y} \land \neg{z})}
      \land \neg{(\neg{x} \land \neg{y} \land z)}$\\
$\Rightarrow (\neg{x} \lor \neg{y} \lor \neg{z}) 
      \land (\neg{x} \lor \neg{y} \lor z) \land (x \lor y \lor \neg{z})$

\end{document}
